notes

Spacetalk/Basic.lean
@@ -15,8 +15,6 @@ namespace Spatium
 
   inductive Op : Ty → Ty → Type
     | plus : Op (.nat × .nat) .nat
-    | minus : Op (.nat × .nat) .nat
-    | mult : Op (.nat × .nat) .nat
 
   inductive Term : Ty → Type
     | const : Nat → Term .nat
@@ -35,8 +33,6 @@ namespace Spatium
 
   @[simp] def Op.denote : Op α β → (α.denote → β.denote)
     | plus => λ (a, b) => a + b
-    | minus => λ (a, b) => a - b
-    | mult => λ (a, b) => a * b
 
   @[simp] def Term.denote : Term ty → ty.denote
     | const x => x
@@ -44,6 +40,21 @@ namespace Spatium
     | range n => List.range n.denote
     | zip a b => List.zip a.denote b.denote
     | map f l => List.map f.denote l.denote
+
+  namespace Example
+    -- A rudimentary a + b example
+    -- where a and b are two streams that range over [0-9]
+    -- and a node c sums the two streams
+    def a : Term (.stream .nat) := .range (.const 10)
+    def b : Term (.stream .nat) := .range (.const 10)
+    def zipper : Term (.stream (.nat × .nat)) := .zip a b
+    def c : Term (.stream .nat) := .map (.op .plus) zipper
+
+    def a_plus_b := (List.zip (List.range 10) (List.range 10)).map (λ (a, b) => a + b)
+
+    example : c.denote = a_plus_b := by
+      simp
+  end Example
 
 end Spatium
 
@@ -54,14 +65,17 @@ namespace VirtFlow
   -- Syntax
 
   inductive Ty
+    | unit
     | nat
     | bool
 
   @[reducible] def Ty.denote : Ty → Type
+    | unit => Unit
     | bool => Bool
     | nat => Nat
 
   inductive NodeOps : List Ty → List Ty → Type
+    | nop : NodeOps α α -- for stateless nodes
     | inc : NodeOps [.nat] [.nat]
     | add : NodeOps [.nat, .nat] [.nat]
     | sub : NodeOps [.nat, .nat] [.nat]
@@ -70,7 +84,18 @@ namespace VirtFlow
     | tail : NodeOps α α.tail
     | comp : NodeOps α β → NodeOps β γ → NodeOps α γ
 
+  -- We choose to denote a List Ty with a tuple instead of a heterogenous list 
+  @[reducible] def ty_list_denote : List Ty → Type
+    | [] => Unit
+    | ty :: [] => ty.denote
+    | ty :: tail => ty.denote × (ty_list_denote tail)
+
   -- Buffer sizes will be modeled later
+  -- Special output fifo?
+  -- Maybe explicitly separate outputs
+  -- Given that one node might not be able to emit N streams
+  -- Find ways to tie back to original program
+  -- conditionally dequeable and enqueable, for reductions
   structure FIFO (num_nodes : Nat) where
     ty : Ty
     producer : Fin num_nodes
@@ -84,11 +109,13 @@ namespace VirtFlow
     let filtered := fifos.toList.filter (·.consumer == id)
     filtered.map (·.ty)
 
+  -- State should need done signals
+  -- Maybe separate state transforms
   structure Node (fifos : Vector (FIFO num_nodes) num_fifos) (id : Fin num_nodes) where
-    state : Ty
-    initial_state : state.denote
-    state_transform : NodeOps [state] [state]
-    ops : NodeOps (state :: (find_inputs fifos id)) (find_outputs fifos id)
+    state : List Ty
+    initial_state : ty_list_denote state
+    state_transform : NodeOps state state
+    pipeline : NodeOps (state ++ (find_inputs fifos id)) (find_outputs fifos id)
 
   -- First node is the initial node and last node is the terminal node
   def NodeList {num_nodes num_fifos : Nat} (fifos : Vector (FIFO num_nodes) num_fifos) :=
@@ -102,12 +129,6 @@ namespace VirtFlow
 
   -- Semantics
 
-  -- We choose to denote a List Ty with a tuple instead of a heterogenous list 
-  @[reducible] def ty_list_denote : List Ty → Type
-    | [] => Unit
-    | ty :: [] => ty.denote
-    | ty :: tail => ty.denote × (ty_list_denote tail)
-
   @[simp] def node_ops_tail_denote (l : ty_list_denote α) : ty_list_denote α.tail :=
     match α with
       | [] => ()
@@ -115,6 +136,7 @@ namespace VirtFlow
       | _ :: _ :: _ => l.snd
   
   @[simp] def NodeOps.denote : NodeOps α β → (ty_list_denote α → ty_list_denote β)
+    | nop => id
     | inc => (· + 1)
     | add => λ (a, b) => a + b
     | sub => λ (a, b) => a - b
